src/Concurrent/BisimReductions.v
@@ -184,7 +184,7 @@ match a with
   match mk_list v2 with
   | Some l =>
     (* NOTE: keep this consistent with the definition in NodeSemantics.v *)
-    match create_result (IApp v1) l, f with
+    match create_result (IApp v1) l 0, f with  (* 0 because FS encoding shouldn't matter here *)
     | Some (r, eff), true =>
       match Π !! ιbase, s with
       (* NOTE: Π !! ιbase is always going to be a dead process where this function is used *)
